Validator/Learning/Compress.lean
@@ -28,7 +28,7 @@ def derive [DecidableEq φ]
   else
     match t with
     | Hedge.Node.mk label children =>
-      let ifexprs: IfExprs n φ (Symbol.nums xs) := Enter.deriveEnter xs
+      let ifexprs: IfExprs n φ (Symbol.nums xs) := Enter.enters xs
       let childxs: Rules n φ (Symbol.nums xs) := IfExpr.evals G Φ ifexprs label
       -- cchildxs = compressed expressions to evaluate on children.
       let ⟨n, cchildxs, indices⟩ := Compress.compress childxs
@@ -36,7 +36,7 @@ def derive [DecidableEq φ]
       let cdchildxs := List.foldl (derive G Φ) cchildxs children
       -- dchildxs = uncompressed derivatives of children.
       let dchildxs := Compress.expand indices cdchildxs
-      LeaveSmart.deriveLeaves xs (Vec.map dchildxs Rule.null)
+      LeaveSmart.leaves xs (Vec.map dchildxs Rule.null)
 
 def derivs [DecidableEq φ]
   (G: Grammar n φ) (Φ : φ → α → Bool)
