Validator/Regex/LeaveMem.lean
@@ -57,12 +57,12 @@ def deriveLeaveM
   match get? memoized key with
   | Option.none =>
     Debug.debug "cache miss"
-    let newvalue := LeaveSmart.deriveLeaves xs ns
+    let newvalue := LeaveSmart.leaves xs ns
     LeaveMem.setLeave (insert memoized key newvalue)
     return newvalue
   | Option.some value =>
     Debug.debug "cache hit"
     return value
 
-instance [DecidableEq σ] [Hashable σ] [Monad m] [Debug m] [MonadExcept String m] [LeaveMem m σ] : LeaveSmart.DeriveLeaveM m σ where
+instance [DecidableEq σ] [Hashable σ] [Monad m] [Debug m] [MonadExcept String m] [LeaveMem m σ] : Leave.DeriveLeaveM m σ where
   deriveLeaveM {l: Nat} (xs: Vec (Regex σ) l) (ns: Vec Bool (Symbol.nums xs)): m (Vec (Regex σ) l) := deriveLeaveM xs ns
