Validator/Regex/Symbol.lean
@@ -67,31 +67,31 @@ def derives {σ: Type} {α: Type} (Φ: σ -> α -> Bool) (rs: Vec (Regex σ) l) 
 -- This gives the predicate control over the evaluation order of α, for example α is a tree, we can first evaluate the same label, before traversing down.
 def derives_preds {σ: Type} {α: Type}
   (ps: {n: Nat} -> Vec σ n -> α -> Vec Bool n) (rs: Vec (Regex σ) l) (a: α): Vec (Regex σ) l :=
-  let symbols: Vec σ (Symbol.nums rs) := Enter.deriveEnter rs
+  let symbols: Vec σ (Symbol.nums rs) := Enter.enters rs
   let pred_results: Vec Bool (Symbol.nums rs) := ps symbols a
-  Leave.deriveLeaves rs pred_results
+  Leave.leaves rs pred_results
 
 def derives_closures {σ: Type}
   (ps: {n: Nat} -> Vec σ n -> Vec Bool n) (rs: Vec (Regex σ) l): Vec (Regex σ) l :=
-  let symbols: Vec σ (Symbol.nums rs) := Enter.deriveEnter rs
+  let symbols: Vec σ (Symbol.nums rs) := Enter.enters rs
   let pred_results: Vec Bool (Symbol.nums rs) := ps symbols
-  Leave.deriveLeaves rs pred_results
+  Leave.leaves rs pred_results
 
 def derives_closures' {σ: Type}
   (ps: {n: Nat} -> Vec σ n -> Vec Bool n) (rs: Vec (Regex σ) l): Vec (Regex σ) l :=
-  Leave.deriveLeaves rs (ps (Enter.deriveEnter rs))
+  Leave.leaves rs (ps (Enter.enters rs))
 
 def derives_closure {σ: Type}
   (p: σ -> Bool) (rs: Vec (Regex σ) l): Vec (Regex σ) l :=
-  let symbols: Vec σ (Symbol.nums rs) := Enter.deriveEnter rs
+  let symbols: Vec σ (Symbol.nums rs) := Enter.enters rs
   let pred_results: Vec Bool (Symbol.nums rs) := Vec.map symbols p
-  Leave.deriveLeaves rs pred_results
+  Leave.leaves rs pred_results
 
 def derive_closure {σ: Type}
   (p: σ -> Bool) (r: Regex σ): Regex σ :=
-  let symbols: Vec σ (Symbol.nums #vec[r]) := Enter.deriveEnter #vec[r]
+  let symbols: Vec σ (Symbol.nums #vec[r]) := Enter.enters #vec[r]
   let pred_results: Vec Bool (Symbol.nums #vec[r]) := Vec.map symbols p
-  let res := (Leave.deriveLeaves #vec[r] pred_results)
+  let res := (Leave.leaves #vec[r] pred_results)
   match res with
   | Vec.cons res' Vec.nil => res'
 
@@ -413,8 +413,8 @@ theorem Symbol_derives_is_derives_preds
   simp only
   rw [<- h]
   unfold derives_preds
-  unfold Leave.deriveLeaves
-  unfold Enter.deriveEnter
+  unfold Leave.leaves
+  unfold Enter.enters
   simp only
 
 theorem Symbol_derives_preds_is_derives_closures
